Main.lean
@@ -2,9 +2,9 @@ import AczelSetTheory.CSets
 
 def main : IO Unit := do
   IO.println "Probando la canonización de un CList 'sucio'."
-  let sucio := CList.mk [CList.uno, CList.cero, CList.uno, CList.cero, CList.cero]
-  let limpio := CList.normalizar sucio
-  let esperado := CList.mk [CList.cero, CList.uno]
+  let sucio := CList.mk [CList.one, CList.zero, CList.one, CList.zero, CList.zero]
+  let limpio := CList.normalize sucio
+  let esperado := CList.mk [CList.zero, CList.one]
   IO.println s!"  Original: {repr sucio}"
   IO.println s!"Normalizado: {repr limpio}"
   IO.println s!"   Esperado: {repr esperado}"
